{
 "cells": [
  {
   "cell_type": "markdown",
   "metadata": {},
   "source": [
    "## III.4 Classical Orthogonal Polynomials\n",
    "\n",
    "Classical orthogonal polynomials are special families of orthogonal polynomials with a number\n",
    "of beautiful properties, for example\n",
    "1. Their derivatives are also OPs\n",
    "2. They are eigenfunctions of simple differential operators\n",
    "\n",
    "As stated above orthogonal polynomials are uniquely defined by the weight\n",
    "$w(x)$ and the constant $k_n$. The classical orthogonal polynomials are:\n",
    "\n",
    "1. Chebyshev polynomials (1st kind) $T_n(x)$: $w(x) = 1/\\sqrt{1-x^2}$ on $[-1,1]$.\n",
    "2.  Chebyshev polynomials (2nd kind) $U_n(x)$: $\\sqrt{1-x^2}$ on $[-1,1]$.\n",
    "2. Legendre polynomials $P_n(x)$: $w(x) = 1$ on $[-1,1]$.\n",
    "4. Ultrapsherical polynomials (my fav!): $C_n^{(λ)}(x)$: $w(x) = (1-x^2)^{λ-1/2}$ on $[-1,1]$, $λ ≠ 0$, $λ > -1/2$.\n",
    "2. Jacobi polynomials: $P_n^{(a,b)}(x)$: $w(x) = (1-x)^a (1+x)^b$ on $[-1,1]$, $a,b > -1$.\n",
    "2. Laguerre polynomials: $L_n(x)$: $w(x) = \\exp(-x)$ on $[0,∞)$.\n",
    "3. Hermite polynomials $H_n(x)$: $w(x) = \\exp(-x^2)$  on $(-∞,∞)$.\n",
    "\n",
    "In the notes we will discuss:\n",
    "\n",
    "1. Chebyshev polynomials: These are closely linked to Fourier series and are one of the most powerful tools in numerics.\n",
    "2. Legendre polynomials: These have no simple closed-form expression but can be defined in terms of a Rodriguez formula, a feature that\n",
    "applies to all other classical families.\n",
    "\n",
    "## 1. Chebyshev\n",
    "\n",
    "**Definition 1 (Chebyshev polynomials, 1st kind)** $T_n(x)$ are orthogonal with respect to $1/\\sqrt{1-x^2}$\n",
    "and satisfy:\n",
    "$$\n",
    "\\begin{align*}\n",
    "T_0(x) &= 1, \\\\\n",
    "T_n(x) &= 2^{n-1} x^n + O(x^{n-1})\n",
    "\\end{align*}\n",
    "$$\n",
    "\n",
    "\n",
    "**Definition 2 (Chebyshev polynomials, 2nd kind)** $U_n(x)$ are orthogonal with respect to $\\sqrt{1-x^2}$.\n",
    "$$\n",
    "U_n(x) = 2^n x^n + O(x^{n-1})\n",
    "$$\n",
    "\n",
    "\n",
    "**Theorem 1 (Chebyshev T are cos)** For $-1 ≤ x ≤ 1$\n",
    "$$\n",
    "T_n(x) = \\cos n\\, {\\rm acos}\\, x.\n",
    "$$\n",
    "In other words\n",
    "$$\n",
    "T_n(\\cos θ) = \\cos n θ.\n",
    "$$\n",
    "\n",
    "\n",
    "**Proof**\n",
    "\n",
    "We need to show that $p_n(x) := \\cos n {\\rm acos}\\, x$ are\n",
    "1. graded polynomials\n",
    "2. orthogonal w.r.t. $1/\\sqrt{1-x^2}$ on $[-1,1]$, and\n",
    "3. have the right normalisation constant $k_n = 2^{n-1}$ for $n = 2,…$.\n",
    "\n",
    "Property (2) follows under a change of variables:\n",
    "$$\n",
    "\\int_{-1}^1 {p_n(x) p_m(x) \\over \\sqrt{1-x^2}} {\\rm d} x =\n",
    "\\int_0^π {\\cos(nθ) \\cos(mθ) \\over \\sqrt{1-\\cos^2 θ}} \\sin θ {\\rm d} θ =\n",
    "\\int_0^π \\cos(nθ) \\cos(mθ) {\\rm d} x = 0\n",
    "$$\n",
    "if $n ≠ m$.\n",
    "\n",
    "To see that they are graded we use the fact that\n",
    "$$\n",
    "x p_n(x) = \\cos θ \\cos n θ = {\\cos(n-1)θ + \\cos(n+1)θ \\over 2} = {p_{n-1}(x) + p_{n+1}(x) \\over 2}\n",
    "$$\n",
    "In other words $p_{n+1}(x) = 2x p_n(x) - p_{n-1}(x)$.\n",
    "Since each time we multiply by $2x$ and $p_0(x) = 1$ we have\n",
    "$$\n",
    "p_n(x) = (2x)^n + O(x^{n-1})\n",
    "$$\n",
    "which completes the proof.\n",
    "\n",
    "∎\n",
    "\n",
    "Buried in the proof is the 3-term recurrence:\n",
    "\n",
    "**Corollary 1 (Chebyshev 3-term recurrence)**\n",
    "$$\n",
    "\\begin{align*}\n",
    "x T_0(x) = T_1(x) \\\\\n",
    "x T_n(x) = {T_{n-1}(x) + T_{n+1}(x) \\over 2}\n",
    "\\end{align*}\n",
    "$$\n",
    "\n",
    "Chebyshev polynomials are particularly powerful as their expansions are cosine series in disguise: for\n",
    "$$\n",
    "f(x) = ∑_{k=0}^∞ f̌_k T_k(x)\n",
    "$$\n",
    "we have\n",
    "$$\n",
    "f(\\cos θ) = ∑_{k=0}^∞ f̌_k \\cos k θ.\n",
    "$$\n",
    "Thus the coefficients can be recovered fast using FFT-based techniques as discussed in the problem sheet.\n",
    "\n",
    "In the problem sheet we will also show the following:\n",
    "\n",
    "**Theorem 2 (Chebyshev U are sin)**\n",
    "For $x = \\cos θ$,\n",
    "$$\n",
    "U_n(x) = {\\sin(n+1) θ \\over \\sin θ}\n",
    "$$\n",
    "which satisfy:\n",
    "$$\n",
    "\\begin{align*}\n",
    "x U_0(x) &= U_1(x)/2 \\\\\n",
    "x U_n(x) &= {U_{n-1}(x) \\over 2} + {U_{n+1}(x) \\over 2}.\n",
    "\\end{align*}\n",
    "$$\n",
    "\n",
    "\n",
    "\n",
    "## 2. Legendre\n",
    "\n",
    "\n",
    "**Definition 3 (Legendre)** Legendre polynomials\n",
    "$P_n(x)$ are orthogonal polynomials with respect to $w(x) = 1$ on $[-1,1]$, with\n",
    "$$\n",
    "k_n = {1 \\over 2^n} \\begin{pmatrix} 2n \\\\ n \\end{pmatrix} =\n",
    "{(2n)! \\over 2^n (n!)^2}\n",
    "$$\n",
    "\n",
    "The reason for this complicated normalisation constant is both historical and\n",
    "that it leads to simpler formulae for recurrence relationships.\n",
    "\n",
    "\n",
    "Classical orthogonal polynomials have _Rodriguez formulae_, defining orthogonal\n",
    "polynomials as high order derivatives of simple functions. In this case we have:\n",
    "\n",
    "**Lemma 1 (Legendre Rodriguez formula)**\n",
    "$$\n",
    "P_n(x) = {1 \\over (-2)^n n!}{{\\rm d}^n \\over {\\rm d} x^n} (1-x^2)^n\n",
    "$$\n",
    "\n",
    "**Proof**\n",
    "We need to verify:\n",
    "1. graded polynomials\n",
    "2. orthogonal to all lower degree polynomials on $[-1,1]$, and\n",
    "3. have the right normalisation constant $k_n = {1 \\over 2^n} \\begin{pmatrix} 2n \\\\ n \\end{pmatrix}$.\n",
    "\n",
    "(1) follows since its a degree $n$ polynomial (the $n$-th derivative of a degree $2n$ polynomial).\n",
    "(2) follows by integration by parts. Note that $(1-x^2)^n$ and its first $n-1$ derivatives vanish at $±1$.\n",
    "If $r_m$ is a degree $m < n$ polynomial we have:\n",
    "$$\n",
    "∫_{-1}^1 {{\\rm d}^n \\over {\\rm d} x^n} (1-x^2)^n r_m(x) {\\rm d}x\n",
    "= -∫_{-1}^1 {{\\rm d}^{n-1} \\over {\\rm d} x^{n-1}} (1-x^2)^n r_m'(x) {\\rm d}x =\n",
    "⋯ = (-)^n ∫_{-1}^1 (1-x^2)^n r_m^{(n)}(x) {\\rm d}x = 0.\n",
    "$$\n",
    "(3) follows since:\n",
    "$$\n",
    "\\begin{align*}\n",
    "{{\\rm d}^n \\over {\\rm d} x^n}[(-)^n x^{2n} + O(x^{2n-1})] &=\n",
    "(-)^n 2n {{\\rm d}^{n-1} \\over {\\rm d} x^{n-1}} x^{2n-1}+ O(x^{2n-1})] \\\\\n",
    "&=\n",
    "(-)^n 2n (2n-1) {{\\rm d}^{n-2} \\over {\\rm d} x^{n-2}} x^{2n-2}+ O(x^{2n-2})] = ⋯ \\\\\n",
    "&= (-)^n 2n (2n-1) ⋯ (n+1) x^n + O(x^{n-1}) =\n",
    "(-)^n {(2n)! \\over n!} x^n + O(x^{n-1})\n",
    "\\end{align*}\n",
    "$$\n",
    "\n",
    "\n",
    "∎\n",
    "\n",
    "This allows us to determine the coefficients $k_n^{(λ)}$ which are useful in proofs. In particular we\n",
    "will use $k_n^{(2)}$:\n",
    "\n",
    "**Lemma 2 (Legendre monomial coefficients)**\n",
    "$$\n",
    "\\begin{align*}\n",
    "P_0(x) &= 1 \\\\\n",
    "P_1(x) &= x \\\\\n",
    "P_n(x) &= \\underbrace{{(2n)! \\over 2^n (n!)^2}}_{k_n} x^n - \\underbrace{(2n-2)! \\over 2^n (n-2)! (n-1)!}_{k_n^{(2)}} x^{n-2} + O(x^{n-4})\n",
    "\\end{align*}\n",
    "$$\n",
    "(Here the $O(x^{n-4})$ is as $x → ∞$, which implies that the term is a polynomial of degree $≤ n-4$. For $n = 2,3$ the $O(x^{n-4})$ term is therefore precisely zero.)\n",
    "\n",
    "**Proof**\n",
    "\n",
    "The $n=0$ and $1$ case are immediate. For the other case we expand $(1-x^2)^n$ to get:\n",
    "$$\n",
    "\\begin{align*}\n",
    "(-)^n {{\\rm d}^n \\over {\\rm d} x^n} (1-x^2)^n &=\n",
    "{{\\rm d}^n \\over {\\rm d} x^n} [ x^{2n} - n x^{2n-2} + O(x^{2n-4})]\\\\\n",
    "&= (2n)⋯(2n-n+1) x^n - n (2n-2)⋯(2n-2-n+1) x^{n-2} + O(x^{n-4}) \\\\\n",
    "&= {(2n)! \\over n!} x^n - {n (2n-2)! \\over (n-2)!} x^{n-2} + O(x^{n-4})\n",
    "\\end{align*}\n",
    "$$\n",
    "Multiplying through by ${1 \\over 2^n (n!)}$ completes the derivation.\n",
    "\n",
    "∎\n",
    "\n",
    "**Theorem 3 (Legendre 3-term recurrence)**\n",
    "$$\n",
    "\\begin{align*}\n",
    "xP_0(x) &= P_1(x) \\\\\n",
    "(2n+1) xP_n(x) &= nP_{n-1}(x) + (n+1)P_{n+1}(x)\n",
    "\\end{align*}\n",
    "$$\n",
    "\n",
    "**Proof**\n",
    "The $n = 0$ case is immediate (since $w(x) = w(-x)$ $a_n = 0$, from PS8).\n",
    "For the other cases we match terms:\n",
    "$$\n",
    "(2n+1)xP_n(x) - n P_{n-1}(x) - (n+1)P_{n+1}(x) = [(2n+1)k_n - (n+1) k_{n+1}] x^{n+1} + [(2n+1) k_n^{(2)} -n k_{n-1} - (n+1) k_{n+1}^{(2)}] x^{n-1} + O(x^{n-3})\n",
    "$$\n",
    "Using the expressions for $k_n$ and $k_n^{(2)}$ above we have (leaving the manipulations as an exercise):\n",
    "$$\n",
    "\\begin{align*}\n",
    "(2n+1)k_n - (n+1) k_{n+1} = {(2n+1)! \\over 2^n (n!)^2} - (n+1) {(2n+2)! \\over 2^{n+1} ((n+1)!)^2} = 0 \\\\\n",
    "(2n+1) k_n^{(2)} -n k_{n-1}  - (n+1) k_{n+1}^{(2)} =  -(2n+1) {(2n-2)! \\over 2^n (n-2)! (n-1)!} - n {(2n-2)! \\over 2^{n-1} ((n-1)!)^2} + (n+1){(2n)! \\over 2^{n+1} (n-1)! n!} = 0\n",
    "\\end{align*}\n",
    "$$\n",
    "Thus\n",
    "$$\n",
    "(2n+1)xP_n(x) - n P_{n-1}(x) - (n+1)P_{n+1}(x) = O(x^{n-3})\n",
    "$$\n",
    "But as it is orthogonal to $P_k(x)$ for $0 ≤ k ≤ n-3$ it must be zero.\n",
    "∎"
   ]
  }
 ],
 "metadata": {
  "kernelspec": {
   "display_name": "Julia 1.8.3",
   "language": "julia",
   "name": "julia-1.8"
  },
  "language_info": {
   "file_extension": ".jl",
   "mimetype": "application/julia",
   "name": "julia",
   "version": "1.8.3"
  }
 },
 "nbformat": 4,
 "nbformat_minor": 2
}
