{
 "cells": [
  {
   "cell_type": "markdown",
   "metadata": {},
   "source": [
    "# MATH50003 Numerical Analysis (2022–23)\n",
    "# Problem Sheet 8\n",
    "\n",
    "\n",
    "\n",
    "This problem sheet explores Fourier expandsions and the Discrete Fourier Transform (DFT).\n",
    "\n",
    "----\n",
    "\n",
    "**Problem 1** Give explicit formulae for $f̂_k$ and $f̂_k^n$ for the following functions:\n",
    "$$\n",
    "\\cos θ, \\cos 4θ, \\sin^4θ, {3 \\over 3 - {\\rm e}^{\\rm i θ}}, {1 \\over 1 - 2{\\rm e}^{\\rm i θ}}\n",
    "$$\n",
    "Hint: You may wish to try the change of variables $z = {\\rm e}^{-{\\rm i}θ}$.\n",
    "\n",
    "**SOLUTION**\n",
    "\n",
    "1. Just expand in complex exponentials to find that\n",
    "$$\n",
    "\\cos θ = {\\exp({\\rm i} θ) + \\exp(-{\\rm i} θ) \\over 2}\n",
    "$$\n",
    "that is $f̂_1 = f̂_{-1} = 1/2$, $f̂_k = 0$ otherwise.\n",
    "Therefore for $p∈ ℤ$ we have\n",
    "$$\n",
    "\\begin{align*}\n",
    "f̂_k^1 &= f̂_1 + f̂_{-1} = 1 \\\\\n",
    "f̂_{2p}^2 &= 0, f̂_{2p+1}^2 = f̂_1 + f̂_{-1} = 1 \\\\\n",
    "f̂_{1+np}^n &= f̂_{-1+np}^n = 1/2, f̂_k^n = 0 \\hbox{otherwise} \\\\\n",
    "\\end{align*}\n",
    "$$\n",
    "2. Similarly\n",
    "$$\n",
    "\\cos 4 θ = {\\exp(4{\\rm i} θ) + \\exp(-4{\\rm i} θ) \\over 2}\n",
    "$$\n",
    "that is $f̂_4 = f̂_{-4} = 1/2$, $f̂_k = 0$ otherwise.\n",
    "Therefore for $p∈ ℤ$ we have\n",
    "$$\n",
    "\\begin{align*}\n",
    "f̂_p^1 &= f̂_4 + f̂_{-4} = 1 \\\\\n",
    "f̂_{2p}^2 &= f̂_4 + f̂_{-4} = 1, f̂_{2p+1}^2 = 0 \\\\\n",
    "f̂_{3p}^3 &= 0, f̂_{3p±1}^3 = f̂_{±4} =1/2 \\\\\n",
    "f̂_{4p}^4 &= f̂_{-4} + f̂_4 = 1, f̂_{4p±1}^4 = 0,  f̂_{4p+2}^4 = 0 \\\\\n",
    "f̂_{5p}^5 &= 0, f̂_{5p+1}^5 = f̂_{-4} = 1/2, f̂_{5p-1}^5 = f̂_{4} = 1/2,  f̂_{5p±2}^5 =0  \\\\\n",
    "f̂_{6p}^6 &=0, f̂_{6p±1}^6 = 0,  f̂_{6p+2}^6 = f̂_{-4} = 1/2,  f̂_{6p-2}^6 = f̂_{4} = 1/2, f̂_{6p+3}^6 =0  \\\\\n",
    "f̂_{7p}^7 &= 0, f̂_{7p±1}^7 = 0,  f̂_{7p±2}^7 = 0, f̂_{7p±3}^7 = f̂_{∓4} = 1/2 \\\\\n",
    "f̂_{8p}^8 &= f̂_{8p±1}^8 = f̂_{8p±2}^8 =  f̂_{8p±3}^8 = 0, f̂_{8p+4}^8 = f̂_4 + f̂_{-4} = 1 \\\\\n",
    "f̂_{k+pn}^n &= f̂_k \\hbox{ for $-4 ≤ k ≤ 4$, 0 otherwise}.\n",
    "\\end{align*}\n",
    "$$\n",
    "3. Here we have:\n",
    "$$\n",
    "(\\sin θ)^4= \\left({\\exp({\\rm i} θ) - \\exp(-{\\rm i} θ) \\over 2 {\\rm i}}\\right)^4\n",
    "= \\left({\\exp(2{\\rm i} θ) -2 + \\exp(-2{\\rm i} θ) \\over -4}\\right)^2\n",
    "= {\\exp(4{\\rm i} θ) -4\\exp(2{\\rm i} θ) +6 -4 \\exp(-2{\\rm i} θ)+\\exp(-2{\\rm i} θ) \\over 16}\n",
    "$$\n",
    "that is $f̂_{-4} = f̂_4 = 1/16$, $f̂_{-2} = f̂_2 = -1/4$, $f_0 = 3/8$, $f̂_k = 0$ otherwise.\n",
    "Therefore for $p∈ ℤ$ we have\n",
    "$$\n",
    "\\begin{align*}\n",
    "f̂_p^1 &=f̂_{-4} + f̂_{-2} + f̂_0 + f̂_2 +  f̂_4 = 0 \\\\\n",
    "f̂_k^2 &= 0 \\\\\n",
    "f̂_{3p}^3 &= f̂_0 = 3/8, f̂_{3p+1}^3 = f̂_{-2} + f̂_4 =-3/16,  f̂_{3p-1}^3 = f̂_{2} + f̂_{-4} =-3/16 \\\\\n",
    "f̂_{4p}^4 &= f̂_0 + f̂_{-4} + f̂_4 = 1/2, f̂_{4p±1}^4 = 0,  f̂_{4p+2}^4 = f̂_{2} + f̂_{-2} =-1/2 \\\\\n",
    "f̂_{5p}^5 &= f̂_0 = 3/8, f̂_{5p+1}^5 = f̂_{-4} = 1/16, f̂_{5p-1}^5 = f̂_{4} = 1/16,  f̂_{5p+2}^5 = f̂_2 = -1/4, f̂_{5p-2}^5 = f̂_{-2} = -1/4  \\\\\n",
    "f̂_{6p}^6 &= f̂_0 = 3/8, f̂_{6p±1}^6 = 0,  f̂_{6p+2}^6 = f̂_2 + f̂_{-4} = -3/16,  f̂_{6p-2}^6 = f̂_{-2} + f̂_{4} = -3/16, f̂_{6p+3}^6 =0  \\\\\n",
    "f̂_{7p}^7 &= f̂_0 = 3/8, f̂_{7p±1}^7 = 0,  f̂_{7p±2}^7 = f̂_{±2} = -1/4, f̂_{7p±3}^7 = f̂_{∓4} = 1/16 \\\\\n",
    "f̂_{8p}^8 &= f̂_0 = 3/8, f̂_{8p±1}^8 = 0,  f̂_{8p±2}^8 = f̂_{±2} = -1/4, f̂_{8p±3}^8 = 0, f̂_{8p+4}^8 = f̂_4 + f̂_{-4} = 1/8 \\\\\n",
    "f̂_{k+pn}^n &= f̂_k \\hbox{ for $-4 ≤ k ≤ 4$, 0 otherwise}.\n",
    "\\end{align*}\n",
    "$$\n",
    "4. Under the change of variables $z = {\\rm e}^{{\\rm i}θ}$ we can use Geoemtric series to determine\n",
    "$$\n",
    "{3 \\over 3 - z} = {1 \\over 1- z/3} = ∑_{k=0}^∞ {z^k \\over 3^k}\n",
    "$$\n",
    "That is $f̂_k = 1/3^k$ for $k ≥ 0$, and $f̂_k = 0$ otherwise.\n",
    "We then have for $0 ≤ k ≤ n-1$\n",
    "$$\n",
    "f̂_{k+pn}^n = ∑_{ℓ=0}^∞ {1 \\over 3^{k+ℓn}} = {1 \\over 3^k} {1 \\over 1 - 1/3^n} = {3^n \\over 3^{n+k} - 3^k}\n",
    "$$\n",
    "5. Now make the change of variables $z = {\\rm e}^{-{\\rm i} θ}$ to get:\n",
    "$$\n",
    "{1 \\over 1 - 2/z} = {1 \\over -2/z} {1 \\over 1 - z/2} = {1 \\over -2/z} ∑_{k=0}^∞ {z^k \\over 2^k}\n",
    "= - ∑_{k=1}^∞ {{\\rm e}^{-{\\rm i} k θ} \\over 2^k}\n",
    "$$\n",
    "That is $f̂_k = -1/2^{-k}$ for $k ≤ -1$ and 0 otherwise.\n",
    "We then have for $-n ≤ k ≤ -1$\n",
    "$$\n",
    "f̂_{k+pn}^n =- ∑_{ℓ=0}^∞ {1 \\over 2^{-k+ℓn}} = -{1 \\over 2^{-k}} {1 \\over 1 - 1/2^n} = -{2^{n+k} \\over 2^n - 1}\n",
    "$$\n",
    "\n",
    "**END**\n",
    "\n",
    "------\n",
    "\n",
    "**Problem 2** Prove that if the first $λ-1$ derivatives $f(θ), f'(θ), …, f^{(λ-1)}(θ)$ \n",
    "are 2π-periodic and $f^{(λ)}$ is uniformly bounded  that\n",
    "$$\n",
    "|f̂_k| = O(|k|^{-λ})\\qquad \\hbox{as $|k| → ∞$}\n",
    "$$\n",
    "Use this to show for the Taylor case ($0 = f̂_{-1} = f̂_{-2} = ⋯$) that\n",
    "$$\n",
    "|f(θ) - ∑_{k=0}^{n-1} f̂_k {\\rm e}^{{\\rm i}kθ}| = O(n^{1-λ})\\qquad \\hbox{as $n → ∞$}\n",
    "$$\n",
    "\n",
    "**SOLUTION**\n",
    "A straightforward application of integration by parts yields the result\n",
    "\n",
    "$$f̂ₖ = \\frac{1}{2π} \\int^{2π}_{0} f(θ) {\\rm e}^{-ikθ} dθ = \\frac{(-i)^λ}{2π k^{λ}} \\int^{2π}_{0} f^{(λ)}(θ) {\\rm e}^{-ikθ} dθ  $$\n",
    "given that $f^{(λ)}$ is uniformly bounded, the second part follows directly from this result\n",
    "\n",
    "$$\n",
    "|∑_{k=n}^{∞} f̂_k {\\rm e}^{{\\rm i}kθ}| ≤ ∑_{k=n}^{∞} |f̂_k | ≤ C ∑_{k=n}^{∞} k^{-λ} \n",
    "$$\n",
    "\n",
    "for some constant $C$.\n",
    "\n",
    "**END**\n",
    "\n",
    "----\n",
    "\n",
    "**Problem 3.1**\n",
    "If $f$ is a trigonometric polynomial  ($f̂_k = 0$ for $|k| > m$) show\n",
    "for $n ≥ 2m+1$ that we can exactly recover $f$:\n",
    "$$\n",
    "f(θ) = \\sum_{k=-m}^m f̂_k^n {\\rm e}^{{\\rm i} k θ}\n",
    "$$\n",
    "\n",
    "**SOLUTION**\n",
    "This follows from\n",
    "$$\n",
    "f̂_k^n = ∑_{p=-∞}^∞ f̂_{k+pn} = f̂_k\n",
    "$$\n",
    "if $-m ≤ k ≤ m$ as if $p > 0$ we have $k + p n ≥ k + 2m+1 ≥ m+1$ hence\n",
    "$f̂_{k+pn} = 0$ and if $k < 0$ we have $k - pn ≤ k -2m-1 ≤ -m-1$ hence\n",
    "$f̂_{k+pn} = 0$.\n",
    "\n",
    "**END**\n",
    "\n",
    "**Problem 3.2** For the general (non-Taylor) case and $n = 2m+1$, prove convergence for\n",
    "$$\n",
    "f_{-m:m}(θ) := ∑_{k=-m}^m f̂_k^n {\\rm e}^{{\\rm i} k θ}\n",
    "$$\n",
    "to $f(θ)$ as $n → ∞$.\n",
    "What is the rate of convergence if the first $λ-1$ derivatives $f(θ), f'(θ), …, f^{(λ-1)}(θ)$ \n",
    "are 2π-periodic and $f^{(λ)}$ is uniformly bounded?\n",
    "\n",
    "**SOLUTION**\n",
    "\n",
    "Observe that by aliasing (see corollary in lecture notes) and triangle inequality we have the following \n",
    "\n",
    "$$ |f̂_k^n - f̂_k|  ≤ \\sum_{p=1}^{∞} (|f̂_{k+pn}|+|f̂_{k-pn}|) $$\n",
    "\n",
    "Using the result from Problem 2 yields\n",
    "\n",
    "$$ |f̂_k^n - f̂_k| ≤ \\frac{C}{n^λ} \\sum_{p=1}^{∞} \\frac{1}{\\left(p + \\frac{k}{n}\\right)^λ} + \\frac{1}{\\left(p - \\frac{k}{n}\\right)^λ} $$\n",
    "\n",
    "now we pick $|q| < \\frac{1}{2}$ (such that the estimate below will hold for both summands above) and construct an integral with convex and monotonocally decreasing integrand such that\n",
    "\n",
    "$$ \\left( p + q \\right)^{-λ} < \\int_{p-\\frac{1}{2}}^{p+\\frac{1}{2}} (x + q)^{-λ} dx $$\n",
    "\n",
    "more over summing over the left-hand side from $1$ to $∞$ yields a bound by the integral:\n",
    "\n",
    "$$ \\int^{∞}_{\\frac{1}{2}} (x + q)^{-λ} dx = \\frac{1}{λ}(\\frac{1}{2} + q)^{- λ + 1}$$\n",
    "\n",
    "Finally let $q = \\pm \\frac{k}{n}$ to achieve the rate of convergence\n",
    "\n",
    "$$ |f̂_k^n - f̂_k| ≤ \\frac{C_{λ}}{ n^{λ}} \\left(  \\left( \\frac{1}{2} + k/n \\right)^{ - λ + 1} + \\left( \\left( \\frac{1}{2} - k/n \\right) \\right)^{- λ +1} \\right)$$\n",
    "\n",
    "where $C_{λ}$ is a constant depending on $λ$. Note that it is indeed important to split the $n$ coefficients equally over the negative and positive coefficients as stated in the notes, due to the estatime we used above.\n",
    "\n",
    "Finally, we have:\n",
    "$$\n",
    "\\begin{align*}\n",
    "|f(θ) - f_{-m:m}(θ)|\n",
    "&= |\\sum_{k=-m}^m {(f̂_k - f̂_k^n)z^k} + \\sum_{k=m+1}^∞ {f̂_k z^k}  + \\sum_{k=-∞}^{-m-1} {f̂_k z^k} | \\\\\n",
    "&\\le \\sum_{k=-m}^m | f̂_k - f̂_k^n | + \\sum_{k=m+1}^∞ |f̂_k| +  \\sum_{k=-∞}^{-m-1} |f̂_k| \\\\\n",
    "&\\le \\sum_{k=-m}^m {\\frac{C_{λ}}{ n^{λ}} \\left( \\left( \\frac{1}{2} + k/n \\right)^{ - λ + 1} + \\left( \\left( \\frac{1}{2} - k/n \\right) \\right)^{- λ +1} \\right)} + \\sum_{k=m+1}^∞ |f̂_k| +  \\sum_{k=-∞}^{-m-1} |f̂_k| \\\\\n",
    "&= \\frac{C_{λ}}{n^{λ}} 2^{λ} + \\sum_{k=m+1}^∞ |f̂_k| +  \\sum_{k=-∞}^{-m-1} |f̂_k|  \\\\\n",
    "&= O(n^{-λ}) + O(n^{1-λ} ) + O(n^{1-λ} ) \\\\\n",
    "&= O(n^{1-λ}) \n",
    "\\end{align*}\n",
    "$$\n",
    "\n",
    "**END**\n",
    "\n",
    "----\n",
    "\n",
    "\n",
    "**Problem 4.1⋆** Show for $0 ≤ k,ℓ ≤ n-1$\n",
    "$$\n",
    "{1 \\over n} \\sum_{j=1}^n \\cos k θ_j \\cos ℓ θ_j = \\begin{cases} 1 & k = ℓ = 0 \\\\\n",
    "                                                  1/2 & k = ℓ \\\\\n",
    "                                                  0 & \\hbox{otherwise}\n",
    "                                                  \\end{cases}\n",
    "$$\n",
    "for $θ_j = π(j-1/2)/n$. Hint: Be careful as the $θ_j$ differ from before, \n",
    "and only cover half the period, $[0,π]$. Using symmetry may help.\n",
    "You may also consider replacing $\\cos$ with \n",
    "complex exponentials:\n",
    "$$\n",
    "\\cos θ = {{\\rm e}^{{\\rm i}θ} + {\\rm e}^{-{\\rm i}θ} \\over 2}.\n",
    "$$\n",
    "\n",
    "\n",
    "**SOLUTION**\n",
    "We have,\n",
    "\n",
    "$$\n",
    "\\begin{align*}\n",
    "\\frac{1}{n}\\sum_{j=1}^n \\cos(kθ_j)\\cos(lθ_j) &= \\frac{1}{4n}\\sum_{j=1}^ne^{i(k+l)θ_j} + e^{-i(k+l)θ_j} + e^{i(k-l)θ_j} + e^{-i(k-l)θ_j} \\\\\n",
    "&=\t\\frac{1}{4n}\\sum_{j=1}^ne^{ia_{kl}θ_j} + e^{-ia_{kl}θ_j} + e^{ib_{kl}θ_j} + e^{-ib_{kl}θ_j},\n",
    "\\end{align*}\n",
    "$$\n",
    "where we have defined $a_{kl} = k+l$ and $b_{kl} = k-l$. Now consider, for $a \\in \\mathbb{Z}$, a $\\neq 2kn$ for some $k \\in \\mathbb{Z}$,\n",
    "$$\n",
    "\\begin{align*}\n",
    "\t\\sum_{j=1}^n e^{iaθ_j} &=\\sum_{j=1}^n e^{iaπ(j-\\frac{1}{2})/n} \\\\\n",
    "\t&=e^{-iaπ/2n}\\sum_{j=1}^n e^{iajπ/n} \\\\\n",
    "\t&=e^{-iaπ/2n}\\sum_{j=1}^n (e^{iaπ/n})^j \\\\\n",
    "\t&=e^{-iaπ/2n} e^{iaπ /n}\\frac{(e^{iaπ /n})^n - 1}{e^{iaπ/n} - 1} \\\\\n",
    "\t&= e^{iaπ/2n} \\frac{e^{iaπ} - 1 }{e^{iaπ / n} - 1},\n",
    "\\end{align*}\n",
    "$$\n",
    "where our assumptions on $a$ ensure that we are not dividing by $0$. Then we have, for $a$ as above,\n",
    "$$\n",
    "\\begin{align*}\n",
    "\t\\sum_{j=1}^n e^{iaθ_j} + e^{-iaθ_j} &= e^{iaπ/2n} \\frac{e^{iaπ} - 1 }{e^{iaπ / n} - 1} + e^{-iaπ/2n} \\frac{e^{-iaπ} - 1 }{e^{-iaπ / n} - 1} \\\\\n",
    "\t&= e^{iaπ/2n} \\frac{e^{iaπ} - 1 }{e^{iaπ / n} - 1} + e^{-iaπ/2n} \\cdot\\frac{e^{iaπ/n}}{e^{iaπ/n}}\\cdot \\frac{e^{-iaπ} - 1 }{e^{-iaπ / n} - 1} \\\\\n",
    "\t&= e^{iaπ/2n} \\frac{e^{iaπ} - 1 }{e^{iaπ / n} - 1} + e^{iaπ/2n}\\frac{e^{-iaπ} - 1}{1 - e^{iaπ/n}} \\\\\n",
    "\t&=e^{iaπ/2n} \\frac{e^{iaπ} - 1 }{e^{iaπ / n} - 1} - e^{iaπ/2n}\\frac{e^{-iaπ} - 1}{e^{iaπ/n} - 1} \\\\\n",
    "\t&= \\frac{e^{iaπ/2n}}{e^{iaπ/n-1}}\\left(e^{iaπ} - 1 - e^{-iaπ} + 1 \\right) \\\\\n",
    "\t&= \\frac{e^{iaπ/2n}}{e^{iaπ/n-1}}\\frac{1}{2i}\\sin(aπ),\n",
    "\\end{align*}\n",
    "$$\n",
    "which is $0$ for $a$ an integer.\n",
    "\n",
    "Now, when $k = l = 0$, we have $a_{kl} = b_{kl} = 0$, and,\n",
    "$$\n",
    "\\frac{1}{n}\\sum_{j=1}^n \\cos(kθ_j)\\cos(lθ_j) = \\frac{1}{4n}\\sum_{j=1}^n (1 + 1 + 1 + 1) = 1.\n",
    "$$\n",
    "When $k = l \\neq 0$, we have $0 < a_{kl} = 2k < 2n$, and $b_{kl} = 0$. Hence,\n",
    "$$\n",
    "\\begin{align*}\n",
    "\t\\frac{1}{n}\\sum_{j=1}^n \\cos(kθ_j)\\cos(lθ_j) &= \\frac{1}{4n}\\sum_{j=1}^n (e^{ia_{kl}θ_j} + e^{-ia_{kl}θ_j} + 1 + 1) \\\\\n",
    "\t&= \\frac{1}{4n}\\left[ \\left(\\sum_{j=1}^n e^{ia_{kl}θ_j} + e^{-ia_{kl}θ_j}\\right) +2n\\right] \\\\\n",
    "\t&= \\frac{1}{2},\n",
    "\\end{align*}\n",
    "$$\n",
    "since $a_{kl}$ meets the conditions for the sum considered above.\n",
    "\n",
    "When $k \\neq l$, we have, $-2n < a_{kl}, b_{kl} <  2n$ and $a_{kl}, b_{kl} \\neq 0$, hence,\n",
    "$$\n",
    "\\begin{align*}\n",
    "\t\\frac{1}{n}\\sum_{j=1}^n \\cos(kθ_j)\\cos(lθ_j) &= \\frac{1}{4n}\\sum_{j=1}^n (e^{ia_{kl}θ_j} + e^{-ia_{kl}θ_j} + e^{ib_{kl}θ_j} + e^{-ib_{kl}θ_j}) \\\\\n",
    "\t&= \\frac{1}{4n} \\left[\\sum_{j=1}^n (e^{ia_{kl}θ_j} + e^{-ia_{kl}θ_j})  + \\sum_{j=1}^n (e^{ib_{kl}θ_j} + e^{-ib_{kl}θ_j} )\\right] \\\\\n",
    "\t&= 0.\n",
    "\\end{align*}\n",
    "$$\n",
    "\n",
    "**END**\n",
    "\n",
    "\n",
    "**Problem 4.2⋆** Consider the Discrete Cosine Transform (DCT)\n",
    "$$\n",
    "C_n := \\begin{bmatrix}\n",
    "\\sqrt{1/n} \\\\\n",
    " & \\sqrt{2/n} \\\\ \n",
    " && ⋱ \\\\\n",
    " &&& \\sqrt{2/n}\n",
    " \\end{bmatrix}\n",
    "\\begin{bmatrix}\n",
    "    1 & ⋯ & 1\\\\\n",
    "    \\cos θ_1 & ⋯ & \\cos θ_n \\\\\n",
    "    ⋮ & ⋱ & ⋮ \\\\\n",
    "    \\cos (n-1)θ_1 & ⋯ & \\cos (n-1)θ_n\n",
    "\\end{bmatrix}\n",
    "$$\n",
    "for $θ_j = π(j-1/2)/n$. Prove that $C_n$ is orthogonal: $C_n^⊤ C_n = C_n C_n^⊤ = I$.\n",
    "Hint: $C_n C_n^⊤ = I$ might be easier to show than $C_n^⊤ C_n = I$ using the previous problem.\n",
    "\n",
    "**SOLUTION**\n",
    "\n",
    "The components of $C$ without the diagonal matrix, which we may call $\\hat{C}$ are\n",
    "$$\n",
    "\\hat{C}_{ij} = \\cos((j-1)θ_{i-1}),\n",
    "$$\n",
    "where $θ_j = π(j-1/2)/n$. Recalling that the elements of matrix multiplication are given by\n",
    "$$\n",
    "(ab)_{ij} := \\sum_{k=1}^n a_{ik} b_{kj}\n",
    "$$\n",
    "we find that\n",
    "$$\n",
    "(\\hat{C}_n \\hat{C}_n^⊤)_{ij} = \\sum_{k=1}^n \\cos((i-1)θ_{k-1}) \\cos((k-1)θ_{j-1}).\n",
    "$$\n",
    "\n",
    "By using the previous problem and the terms on the diagonal matrices which ensure that the $1/2$ terms become $1$ we know how to compute all of these entries and find that it is the identity.\n",
    "\n",
    "Here is a computer-based demonstration:"
   ]
  },
  {
   "cell_type": "code",
   "execution_count": 1,
   "metadata": {
    "execution": {
     "iopub.execute_input": "2023-04-19T14:28:59.775000Z",
     "iopub.status.busy": "2023-04-19T14:28:59.155000Z",
     "iopub.status.idle": "2023-04-19T14:29:02.692000Z",
     "shell.execute_reply": "2023-04-19T14:29:02.668000Z"
    }
   },
   "outputs": [
    {
     "data": {
      "text/plain": [
       "10×10 Matrix{Float64}:\n",
       "  1.0           3.18525e-17  -1.9692e-17   …  -1.04161e-18   1.59817e-16\n",
       "  3.18525e-17   1.0           3.15615e-17      1.94168e-16  -3.39467e-16\n",
       " -1.9692e-17    3.15615e-17   1.0              3.4151e-17    4.29005e-17\n",
       "  1.46173e-17   6.18906e-17  -8.71939e-17     -4.8386e-16    2.37214e-16\n",
       " -3.83754e-17   1.23093e-16  -7.59471e-17     -5.04681e-17   3.96805e-16\n",
       "  1.29409e-16  -1.73389e-16   2.77887e-17  …   3.22809e-16  -8.83356e-16\n",
       "  1.81485e-16  -2.80487e-16   7.24884e-17      4.9429e-16    3.05676e-16\n",
       "  2.77165e-17  -8.61478e-17   3.11149e-16      2.14724e-16  -2.17458e-16\n",
       " -1.04161e-18   1.94168e-16   3.4151e-17       1.0          -7.06392e-18\n",
       "  1.59817e-16  -3.39467e-16   4.29005e-17     -7.06392e-18   1.0"
      ]
     },
     "execution_count": 1,
     "metadata": {},
     "output_type": "execute_result"
    }
   ],
   "source": [
    "using LinearAlgebra\n",
    "n = 10\n",
    "θ = range(π/(2n); step=π/n, length=n) # n evenly spaced points starting at π/(2n) with step size π/n\n",
    "C = Diagonal([1/sqrt(n); fill(sqrt(2/n), n-1)]) * [cos((k-1)*θ[j]) for k=1:n, j=1:n]\n",
    "C'C"
   ]
  },
  {
   "cell_type": "markdown",
   "metadata": {},
   "source": [
    "**END**"
   ]
  }
 ],
 "metadata": {
  "kernelspec": {
   "display_name": "Julia 1.9.0",
   "language": "julia",
   "name": "julia-1.9"
  },
  "language_info": {
   "file_extension": ".jl",
   "mimetype": "application/julia",
   "name": "julia",
   "version": "1.9.0"
  }
 },
 "nbformat": 4,
 "nbformat_minor": 2
}
